
The last step transforms any program specification to the 
\emph{modular polynomial equation entailment} problem which decides
whether 
\[\forall \vx.
  \bigwedge\limits_i e_i (\vx) = e'_i (\vx) \wedge
  \bigwedge\limits_j f_j (\vx) \equiv f'_j (\vx) \mod n_j
  \implies
  \bigwedge\limits_k g_k (\vx) = g'_k (\vx) \wedge
  \bigwedge\limits_l   h_l (\vx) \equiv h'_l (\vx) \mod m_l
\]
with 
$e_i (\vx), e'_i (\vx), f_j (\vx), f'_j (\vx),
 g_k (\vx), g'_k (\vx), h_l (\vx), h'_l (\vx) \in \bbfZ[\vx]$
for every $i, j, k, l$.

\begin{algorithm}
  \begin{algorithmic}[1]
    \Function{StatementToPolyEQ}{$s$}
    \Match{$s$}
      \Case{$v \leftarrow e$}
        \Return $v = e$
      \EndCase
      \Case{$v_h, v_l \leftarrow \dslcode{Split}(e, n)$}
        \Return $v_l + v_h \times 2^n = e$
      \EndCase
    \EndMatch
    \EndFunction
  \end{algorithmic}
  \caption{Polynomial Equation Transformation for Statements}
\end{algorithm}

\begin{algorithm}
  \begin{algorithmic}[1]
    \Function{ProgramToPolyEQ}{$p$}
    \Match{$p$}
      \Case{$\epsilon$} \Return $\top$ \EndCase
      \Case{$s; pp$}
        \Return \Call{StatementToPolyEQ} ($s$) $\wedge$
                \Call{ProgramToPolyEQ} ($pp$)
      \EndCase
    \EndMatch
    \EndFunction
  \end{algorithmic}
  \caption{Polynomial Equation Transformation for Programs}
  \label{algorithm:programtoq}
\end{algorithm}

\begin{definition}
  A program is \emph{well-formed} if
  \begin{itemize}
  \item for every $v_h, v_l \leftarrow \dslcode{Split}(e, n)$, $v_h
    \neq v_l$; and
  \item every variable must be assigned to a value before being used.
  \end{itemize}
\end{definition}

\begin{theorem}
  \label{theorem:program-to-q-soundness}
  Let $q, q' \in Q$ and $p \in P$.
  Suppose $\valueof{q \wedge \textmd{\textit{ProgramToQ}}(p)}_\nu$
  implies $\valueof{q'}_\nu$ for every valuation $\nu$. 
  Then $\cond{q}$ $p$ $\cond{q'}$.
\end{theorem}

Recall the definition of $Q$. By
Theorem~\ref{theorem:program-to-q-soundness}, it remains to establish
that for every $\vec{x} \in \bbfZ^{|\vec{x}|}$, 
\[
  \bigwedge\limits_i e_i (\vec{x}) = e'_i (\vec{x}) \wedge
  \bigwedge\limits_j f_j (\vec{x}) \equiv f'_j (\vec{x}) \mod n_j
  \implies
  \bigwedge\limits_k g_k (\vec{x}) = g'_k (\vec{x}) \wedge
  \bigwedge\limits_l   h_l (\vec{x}) \equiv h'_l (\vec{x}) \mod m_l
\]
where
$e_i (\vec{x}), e'_i (\vec{x}), f_j (\vec{x}), f'_j (\vec{x}),
 g_k (\vec{x}), g'_k (\vec{x}), h_l (\vec{x}), h'_l (\vec{x})$
are multivariant polynomials over $\vec{x}$, and
$n_j, m_l \in \bbfN $. Since the conclusion is a conjunction of
(modulo) equations, we will prove one conjunct at a time. That is, for
every $\vec{x} \in \bbfZ^{|\vec{x}|}$, 
\[
  \bigwedge\limits_i e_i (\vec{x}) = e'_i (\vec{x}) \wedge
  \bigwedge\limits_j f_j (\vec{x}) \equiv f'_j (\vec{x}) \mod n_j
  \implies
  g (\vec{x}) = g' (\vec{x})
\] where $g (\vec{x})$ and $g' (\vec{x})$ are multivariant polynomials
over $\vec{x}$. Or,
\[
  \bigwedge\limits_i e_i (\vec{x}) = e'_i (\vec{x}) \wedge
  \bigwedge\limits_j f_j (\vec{x}) \equiv f'_j (\vec{x}) \mod n_j
  \implies
  h (\vec{x}) \equiv h' (\vec{x}) \mod m
\] where $h (\vec{x})$ and $h' (\vec{x})$ are multivariant polynomials
over $\vec{x}$ and $m \in \bbfN$.
